src/SDK/AlgorithmSuite.dfy
@@ -14,9 +14,7 @@ module AlgorithmSuite {
 
   newtype ID = x | x in validIDs witness 0x0014
   {
-    function method KeyLength(): nat
-      ensures KeyLength() < 0x100
-    {
+    function method KeyLength(): nat {
       Suite[this].params.keyLen as nat
     }
 
